\documentclass{article}
\usepackage{amsmath}
\usepackage{amsfonts}
\usepackage{minted}
\usepackage{fancyvrb}
\title{Intro to Computer Science Assignment 2}
\date{2017-09-20}
\author{Yiping Deng}
\begin{document}
\maketitle
\paragraph{6.1}
Giving two boolean variable $P,Q$\\
By truth table, we have $ P \to Q = \neg P \lor Q $
\begin{align*}
  P \lor Q = \neg \neg P \lor Q = \neg P \to Q \\
  P \land Q = \neg (\neg P \lor \neg Q) = \neg( \neg \neg P \to \neg Q) = \neg (P \to \neg Q)
\end{align*}


\paragraph{6.2}
\subparagraph{1)}
Truth table proof:
\inputminted{text}{table1.md}
\newpage
\inputminted{text}{table2.md}
\textbf{So, 2}
\subparagraph{2)}
DNF form:
\begin{align*}
    \varphi(M, N, P, Q, R, S) &= \\
    &= ((\neg (P \lor Q \lor R \lor S)) \lor (P \land Q \land \land R \land S))) \land M \land \neg N \\
    &= (\neg P \land \neg Q \land \neg R \land \neg S \land M \land \neg N) \lor (P \land Q \land R \land S \land M \land \neg N) \\
\end{align*}

\subparagraph{3)}
\begin{align*}
  \varphi(M, N, P, Q, R, S) &= (\neg P \lor Q) \land (\neg Q \lor R) \land ( \neg R \lor S ) \land (\neg S \lor P) \land M \land \neg N \\
  (\neg P \lor Q) \land (\neg Q \lor R) &= ((\neg P \lor Q) \land \neg Q ) \lor ((\neg P \lor Q) \land R) \\
  &= (\neg P \land \neg Q) \lor (Q \land \neg Q) \lor ((\neg P \lor Q) \land R) \\
  &= (\neg P \land \neg Q) \lor 0 \lor ((\neg P \lor Q) \land R)\\
  &= \neg (P \lor Q) \lor ((\neg P \lor Q) \land R)\\
  (\neg R \lor S) \land (\neg S \lor P) &= \neg (R \lor S) \lor ((\neg R \lor S) \land P) \\
  &(\neg (R \lor S) \lor ((\neg R \lor S) \land P)) \land (\neg (P \lor Q) \lor ((\neg P \lor Q) \land R)) \\
  &= (\neg (P \lor Q \lor R \lor S)  \\
  &\lor ((\neg R \lor S) \land P) \land \neg (P \lor Q))  \\
  &\lor (\neg (R \lor S) \land ((\neg P \lor Q) \land R)) \\
  &\lor ( (\neg R \lor S) \land P) \land ((\neg P \lor Q) \land R)) \\
  &= (\neg (P \lor Q \lor R \lor S)  \\
  &\lor ( (\neg R \lor S) \land P) \land ((\neg P \lor Q) \land R)) \\
  &= (\neg (P \lor Q \lor R \lor S)  \\
  & \lor ( (\neg R \lor S) \land (\neg P \lor Q) \land R \land P)) \\
  &= (\neg (P \lor Q \lor R \lor S) \lor (P \land Q \land R \land S) \\
  \varphi(M, N, P, Q, R, S) &= (\neg (R \lor S) \lor ((\neg R \lor S) \land P)) \land (\neg (P \lor Q) \lor ((\neg P \lor Q) \land R)) \land M \land \neg N \\
  &= ((\neg (P \lor Q \lor R \lor S)) \lor (P \land Q \land \land R \land S))) \land M \land \neg N \\
  &= (\neg P \land \neg Q \land \neg R \land \neg S \land M \land \neg N) \lor (P \land Q \land R \land S \land M \land \neg N) \\
\end{align*}

\paragraph{6.3}
\inputminted{haskell}{code.hs}
\end{document}
