\documentclass{article}
\usepackage{amsmath}
\usepackage{amsfonts}
\usepackage{minted}
\title{Intro to Computer Science Assignment 2}
\date{2017-09-20}
\author{Yiping Deng}
\begin{document}
\maketitle
\paragraph{Problem 2.1} \hfill \break
Proof by its cotrapositive: \hfill \break
Lemma: If n is not divisible by 3, then $n^2$ is not divisible by 3. \hfill \break
\textbf{Proof} :  \hfill \break
3 is a prime number, n is not divisible by 3$\implies $ 3 is not a factor of n $\implies $ 3 is not a factor of $ n \cdot n = n^2 \implies$ n is not divisible by 3. \hfill \break

\paragraph{Problem 2.2}
Lemma: $ 0^3 + 1^3 + 2^3 + ... + n^3 = \sum_{i=0}^{n} i^3 = [\frac{n(n + 1)}{2}]^2$ \hfill \break
\textbf{Proof by induction:} \\
Basis:
\begin{align}
 n = 0 \\
 \implies \sum_{i=0}^{n} i^3 = 0^3 = 3 \\
[\frac{n(n + 1)}{2}]^2 = [\frac{0(0 + 1)}{2}]^2 = 0 \\
\implies \sum_{i=0}^{n} i^3 = [\frac{n(n + 1)}{2}]^2, n = 0
\end{align}
\hfill \break \break
Inductive Proof: Assume lemma holds for $n = k \implies $
\begin{align}
\sum_{i=0}^{k} i^3 =  [\frac{k(k + 1)}{2}]^2 \implies
\sum_{i=0}^{k + 1} i^3
&= \sum_{i=0}^{k} i^3 + (k + 1)^3
= [\frac{k(k + 1)}{2}]^2 + (k + 1)^3
\\& = \frac{k^2(k + 1)^2}{4}+ (k + 1)^3
\\&= \frac{k^2(k + 1)^2}{4} + \frac{(4k+4)(k+1)^2}{4}
\\&= \frac{(k^2 + 4k + 4)(k+1)^2}{4}
\\&= \frac{(k +2 )^2 (k + 1)^2}{4}
\\&= [\frac{(k + 1)(k + 2)}{2}]^2
\end{align}
\end{document}
